prove binary search range function call

theories/binary_search_range_verif.v
@@ -9,12 +9,10 @@ Definition Vprog : varspecs.  mk_varspecs prog. Defined.
 Definition binary_search_range_spec :=
  DECLARE _binary_search_range
   WITH a: val, sh : share, contents : list Z, from : Z, to : Z, key : Z
-  PRE [ tptr tint, tint, tint ]
+  PRE [ tptr tint, tint, tint, tint ]
           PROP (readable_share sh;
-                0 <= from;
-                from <= to;
-                to <= Zlength contents;
-                Zlength contents <= Int.max_signed;
+                0 <= from <= to;
+                to <= Zlength contents <= Int.max_signed;
                 Int.min_signed <= key <= Int.max_signed;
                 Forall (fun x => Int.min_signed <= x <= Int.max_signed) (sublist from to contents);
                 sorted (sublist from to contents))
@@ -26,6 +24,17 @@ Definition binary_search_range_spec :=
                else insertion_point (-i - 1) (sublist from to contents) key from to)
          RETURN (Vint (Int.repr i))
          SEP (data_at sh (tarray tint (Zlength contents)) (map Vint (map Int.repr contents)) a).
+
+Definition binary_search_range_while_spec a sh contents from to key :=
+EX low : Z, EX high : Z,
+ PROP (from <= low <= to;
+       Int.min_signed <= high < to;
+       In key contents -> In key (sublist low (high + 1) contents);
+       ~ In key contents ->
+        Forall (fun x => x < key) (sublist from low contents) /\
+        Forall (fun x => key < x) (sublist (high + 1) to contents))
+ LOCAL (temp _a a; temp _low (Vint (Int.repr low)); temp _high (Vint (Int.repr high)); temp _key (Vint (Int.repr key)))
+ SEP (data_at sh (tarray tint (Zlength contents)) (map Vint (map Int.repr contents)) a).
 
 Definition binary_search_spec :=
  DECLARE _binary_search
@@ -45,3 +54,56 @@ Definition binary_search_spec :=
                else insertion_point (-i - 1) contents key 0 (Zlength contents))
          RETURN (Vint (Int.repr i))
          SEP (data_at sh (tarray tint (Zlength contents)) (map Vint (map Int.repr contents)) a).
+
+Definition main_spec :=
+ DECLARE _main
+  WITH gv: globals
+  PRE  [] main_pre prog tt gv
+  POST [ tint ] main_post prog gv.
+
+Definition Gprog : funspecs := ltac:(with_library prog [binary_search_range_spec; binary_search_spec; main_spec]).
+
+Lemma body_binary_search_range: semax_body Vprog Gprog f_binary_search_range binary_search_range_spec.
+Proof.
+start_function.
+Admitted.
+
+Lemma body_binary_search: semax_body Vprog Gprog f_binary_search binary_search_spec.
+Proof.
+start_function.
+forward_call (a, sh, contents, 0, len, key).
+- pose proof (Zlength_nonneg contents) as Hlen.
+  rewrite H0.
+  split; auto; split; [lia|]; split; [lia|]; split; auto; split.
+  * autorewrite with sublist; assumption.
+  * autorewrite with sublist; assumption.
+- Intro res.
+  forward.
+  revert H4.
+  autorewrite with sublist.
+  case (in_dec _ _ _); intros; Exists res; entailer!.
+Qed.
+
+Definition four_contents := [1; 2; 3; 4].
+
+Lemma body_main : semax_body Vprog Gprog f_main main_spec.
+Proof.
+  start_function.
+  forward_call (gv _four,Ews,four_contents,4,3).
+  { split. auto.
+    change (Zlength four_contents) with 4.
+    repeat constructor; computable.
+  }
+  Intro r; forward.
+Qed.
+
+Existing Instance NullExtension.Espec.
+
+Lemma prog_correct:
+  semax_prog prog tt Vprog Gprog.
+Proof.
+prove_semax_prog.
+semax_func_cons body_binary_search_range.
+semax_func_cons body_binary_search.
+semax_func_cons body_main.
+Qed.
